src/ReactorModel/Determinism/ChangeStep.lean
@@ -1,41 +1,39 @@
-import ReactorModel.Determinism.ChangeEquiv
+import ReactorModel.Execution
 
 open Classical
 
 namespace Execution
+namespace ChangeStep
 
-theorem ChangeStep.preserves_progress (e : s₁ -[c]→ s₂) : s₁.progress = s₂.progress := by
+theorem preserves_progress (e : s₁ -[c]→ s₂) : s₁.progress = s₂.progress := by
   cases e <;> rfl
 
-theorem ChangeStep.preserves_tag (e : s₁ -[c]→ s₂) : s₁.tag = s₂.tag := by
+theorem preserves_tag (e : s₁ -[c]→ s₂) : s₁.tag = s₂.tag := by
   cases e <;> rfl
 
-theorem ChangeStep.preserves_rcns {i : ID} (e : s₁ -[c]→ s₂) :
-    s₁.rtr.obj? .rcn i = s₂.rtr.obj? .rcn i := by
+theorem preserves_rcns {i : ID} (e : s₁ -[c]→ s₂) : s₁.rtr.obj? .rcn i = s₂.rtr.obj? .rcn i := by
   cases e <;> first | rfl | simp [Reactor.Update.preserves_ne_cmp_or_id ‹_›]
 
-theorem ChangeStep.equiv (e : s₁ -[c]→ s₂) : s₁.rtr ≈ s₂.rtr := by
+theorem equiv (e : s₁ -[c]→ s₂) : s₁.rtr ≈ s₂.rtr := by
   cases e 
   case' port h, state h, action h => exact h.equiv
   all_goals exact .refl 
 
-theorem ChangeStep.preserves_unchanged_port 
-    (e : s₁ -[c]→ s₂) (h : ¬c.obj.IsPort i := by exact (nomatch ·)) :
+theorem preserves_unchanged_port (e : s₁ -[c]→ s₂) (h : ¬c.obj.IsPort i := by exact (nomatch ·)) :
     s₁.rtr.obj? .prt i = s₂.rtr.obj? .prt i := by
   cases e
   case port u => simp [Change.IsPort.iff_id_eq] at h; exact u.preserves_ne_id h
   case' state u, action u => exact u.preserves_ne_cmp
   all_goals rfl
 
-theorem ChangeStep.preserves_unchanged_state 
-    (e : s₁ -[c]→ s₂) (h : ¬c.obj.IsState i := by exact (nomatch ·)) : 
+theorem preserves_unchanged_state (e : s₁ -[c]→ s₂) (h : ¬c.obj.IsState i := by exact (nomatch ·)) : 
     s₁.rtr.obj? .stv i = s₂.rtr.obj? .stv i := by
   cases e
   case state u => simp [Change.IsState.iff_id_eq] at h; exact u.preserves_ne_id h
   case' action u, port u => exact u.preserves_ne_cmp
   all_goals rfl
 
-theorem ChangeStep.preserves_unchanged_action 
+theorem preserves_unchanged_action 
     (e : s₁ -[c]→ s₂) (h : ¬c.obj.IsAction i := by exact (nomatch ·)) : 
     s₁.rtr.obj? .act i = s₂.rtr.obj? .act i := by
   cases e 
@@ -43,29 +41,31 @@ theorem ChangeStep.preserves_unchanged_action
   case' state u, port u => exact u.preserves_ne_cmp 
   all_goals rfl
 
-theorem ChangeStep.port_change {i : ID} (h : s₁.rtr.obj? .prt i = some p) :
+theorem port_change {i : ID} (h : s₁.rtr.obj? .prt i = some p) :
     (s₁ -[⟨rcn, .port i v⟩]→ s₂) → s₂.rtr.obj? .prt i = some { p with val := v }
   | port u => by
     have ⟨_, h₁, h₂⟩ := u.change'
     injection h ▸ h₁ with h₁
     simp [h₁, h₂]
 
-theorem ChangeStep.action_change {i : ID} (h : s₁.rtr.obj? .act i = some a) :
+theorem state_change {i : ID} : (s₁ -[⟨rcn, .state i v⟩]→ s₂) → s₂.rtr.obj? .stv i = some v
+  | state u => u.change'.choose_spec.right
+
+theorem action_change {i : ID} (h : s₁.rtr.obj? .act i = some a) :
     (s₁ -[⟨rcn, .action i t v⟩]→ s₂) → s₂.rtr.obj? .act i = some (schedule a t v)
   | action u => by
     have ⟨_, h₁, h₂⟩ := u.change'
     injection h ▸ h₁ with h₁
     simp [h₁, h₂]
 
-theorem ChangeStep.port_preserves_port_role {j : ID} 
+theorem port_preserves_port_role {j : ID} 
     (e : s₁ -[⟨rcn, .port i v⟩]→ s₂) (h : s₁.rtr.obj? .prt j = some p) :
     ∃ v, s₂.rtr.obj? .prt j = some { p with val := v } :=
-  if hi : j = i
+  if hi : i = j
   then ⟨v, hi ▸ e.port_change (hi ▸ h)⟩ 
   else ⟨_, e.preserves_unchanged_port (Change.IsPort.iff_id_eq.not.mpr hi) ▸ h⟩ 
       
-theorem ChangeStep.preserves_port_role {i : ID} 
-    (e : s₁ -[⟨rcn, c⟩]→ s₂) (h : s₁.rtr.obj? .prt i = some p) :
+theorem preserves_port_role {i : ID} (e : s₁ -[⟨rcn, c⟩]→ s₂) (h : s₁.rtr.obj? .prt i = some p) :
     ∃ v, s₂.rtr.obj? .prt i = some { p with val := v } := by
   cases c
   case port => exact e.port_preserves_port_role h
@@ -73,43 +73,52 @@ theorem ChangeStep.preserves_port_role {i : ID}
     simp [←e.preserves_unchanged_port (i := i), h]
     exists p.val
 
-theorem ChangeStep.preserves_same_action_at_unchanged_times
+theorem preserves_same_action_at_unchanged_times
     (e : s₁ -[⟨rcn, .action i t v⟩]→ s₂) (ht : t ≠ t') 
     (ho₁ : s₁.rtr.obj? .act i = some a₁) (ho₂ : s₂.rtr.obj? .act i = some a₂) :
     a₁ ⟨t', m⟩ = a₂ ⟨t', m⟩ := by
   injection e.action_change ho₁ ▸ ho₂ with h
   rw [←h, schedule_preserves_unchanged_time ht]  
 
+theorem action_preserves_action_at_unchanged_times
+    (e : s₁ -[⟨rcn, .action i t v⟩]→ s₂) (hc : i ≠ j ∨ t ≠ t') 
+    (ho₁ : s₁.rtr.obj? .act j = some a₁) (ho₂ : s₂.rtr.obj? .act j = some a₂) :
+    a₁ ⟨t', m⟩ = a₂ ⟨t', m⟩ := by
+  by_cases hi : i = j
+  case neg =>
+    have h := e.preserves_unchanged_action (i := j) (Change.IsAction.iff_id_eq.not.mpr hi) 
+    injection ho₁ ▸ ho₂ ▸ h with h
+    simp [h]
+  case pos =>
+    have ht := hc.resolve_left (not_not.mpr hi)
+    exact e.preserves_same_action_at_unchanged_times ht (hi ▸ ho₁) (hi ▸ ho₂)
+
 -- Note: `ho₁` and `e` imply `ho₂`.
-theorem ChangeStep.preserves_action_at_unchanged_times
+theorem preserves_action_at_unchanged_times
     (e : s₁ -[⟨rcn, c⟩]→ s₂) (hc : ¬c.IsActionAt i t) 
     (ho₁ : s₁.rtr.obj? .act i = some a₁) (ho₂ : s₂.rtr.obj? .act i = some a₂) :
   a₁ ⟨t, m⟩ = a₂ ⟨t, m⟩ := by
   cases c
   case action j t v =>
-    by_cases hi : i = j
-    case neg =>
-      have h := e.preserves_unchanged_action (i := i) (Change.IsAction.iff_id_eq.not.mpr hi) 
-      injection ho₁ ▸ ho₂ ▸ h with h
-      simp [h]
-    case pos =>
-      have ht := Change.not_IsActionAt_eq_ids_to_ne_time (hi ▸ hc)
-      exact e.preserves_same_action_at_unchanged_times ht (hi ▸ ho₁) (hi ▸ ho₂)
+    have ht := Change.not_IsActionAt_ne_ids_or_ne_time hc
+    exact e.action_preserves_action_at_unchanged_times ht ho₁ ho₂
   all_goals
     injection ho₁ ▸ ho₂ ▸ e.preserves_unchanged_action (i := i) with h
     simp [h]
 
 -- TODO: Check if this is still needed after cleaning up `ChangeListStep.equiv_changes_eq_result`.
-theorem ChangeStep.port_change_mem_rtr : 
-    (s -[⟨rcn, .port i v⟩]→ s') → ∃ p, s.rtr.obj? .prt i = some p
+theorem port_change_mem_rtr : (s -[⟨rcn, .port i v⟩]→ s') → ∃ p, s.rtr.obj? .prt i = some p
   | .port u => u.obj?_target
 
-theorem ChangeStep.context_agnostic (e : s₁ -[c]→ s) (h : s₁.rtr = s₂.rtr) :
-  s₂ -[c]→ { s with tag := s₂.tag, progress := s₂.progress } := by
+theorem context_agnostic (e : s₁ -[c]→ s) (h : s₁.rtr = s₂.rtr) :
+    s₂ -[c]→ { s with tag := s₂.tag, progress := s₂.progress } := by
   cases e
   all_goals 
     rw [h] at * 
     constructor <;> assumption
 
-theorem ChangeStep.determinisic (e₁ : s -[c]→ s₁) (e₂ : s -[c]→ s₂) : s₁ = s₂ := by
+theorem deterministic (e₁ : s -[c]→ s₁) (e₂ : s -[c]→ s₂) : s₁ = s₂ := by
   cases e₁ <;> cases e₂ <;> simp <;> try apply Reactor.Update.unique' ‹_› ‹_› 
+
+end ChangeStep
+end Execution
